Tactics/ArmConstr.lean
@@ -20,6 +20,7 @@ This is inspired by `simp_arith`, especially the following files:
 -/
 
 import Arm.Exec
+import Arm.FromMathlib
 
 namespace ArmConstr
 
@@ -58,15 +59,20 @@ def StateVar.denote (ctx : StateContext) (v : StateVar) : ArmState :=
   ctx.getD v ArmState.default
 
 /--
-Denote `GPRVal v`.
-
-If `v` is a variable then look it up in the `GPRValContext`. Else if `v` is
-`r_gpr i`, then look up the `i`th register in `prev_s`.
+Denote `GPRVal v` over `ArmState prev_s`. That is, if `v` is a variable then
+look it up in the `GPRValContext`. Else if `v` is `r_gpr i`, then look up the
+`i`th register in `prev_s`.
 -/
 def GPRVal.denote (ctx : GPRValContext) (v : GPRVal) (prev_s : ArmState) : BitVec 64 :=
   match v with
   | var i => ctx.getD i 0
   | r_gpr i => r (.GPR i) prev_s
+
+@[local simp]
+theorem GPRVal.denote_of_var :
+  GPRVal.denote ctx (GPRVal.var v) s = ctx.getD v 0 := by
+  simp [GPRVal.denote]
+  done
 
 /--
 Datastructure that characterizes all the updates that can be made to an
@@ -93,19 +99,23 @@ instance : Decidable (Update.regEq x y) :=
     | .w_gpr i _, .w_gpr j _ => i = j)
 
 /--
-Is the register index of update `x` less than that of `y`?
+Is the register index of update `x` less than or equal to that of `y`?
 -/
-def Update.regIndexLt (x y : Update) : Bool :=
+def Update.regIndexLe (x y : Update) : Bool :=
   match x, y with
-  | w_gpr i _, w_gpr j _ => i < j
+  | w_gpr i _, w_gpr j _ => i <= j
 
--- instance : Decidable (Update.regIndexLt x y) :=
-  -- inferInstanceAs (Decidable <|
-    -- match x, y with
-    -- | Update.w_gpr i _, Update.w_gpr j _ => i < j)
---
--- def Update.regIndexLtBool (x y : Update) : Bool :=
-  -- decide (x.regIndexLt y)
+theorem Update.regIndexLe_trans (a b c : Update)
+  (h1 : Update.regIndexLe a b)
+  (h2 : Update.regIndexLe b c) :
+  Update.regIndexLe a c := by
+  simp_all [Update.regIndexLe]
+  exact BitVec.le_trans h1 h2
+
+theorem Update.regIndexLe_total (a b : Update) :
+  Update.regIndexLe a b || Update.regIndexLe b a := by
+  simp_all [Update.regIndexLe]
+  exact BitVec.le_total a.1 b.1
 
 /--
 Datastructure to represent expressions characterizing the following state
@@ -123,21 +133,108 @@ deriving DecidableEq, Repr, Inhabited
 /--
 Map updates `us` to state `prev_state` to an `ArmState`.
 -/
-def Expr.writes.denote (ctx : Context) (us : Updates) (prev_state : StateVar)
+def Expr.denote_writes (ctx : Context) (us : Updates) (prev_state : StateVar)
   : ArmState :=
   match us with
   | [] => StateVar.denote ctx.state prev_state
   | Update.w_gpr i v :: rest =>
     w (.GPR i)
       (GPRVal.denote ctx.gpr v (StateVar.denote ctx.state prev_state))
-      (Expr.writes.denote ctx rest prev_state)
+      (Expr.denote_writes ctx rest prev_state)
+
+@[local simp]
+theorem denote_writes_empty :
+  Expr.denote_writes ctx [] prev_state = StateVar.denote ctx.state prev_state := by
+  simp only [Expr.denote_writes]
+
+@[local simp]
+theorem denote_writes_cons :
+  Expr.denote_writes ctx (e :: us) prev_state =
+  w (StateField.GPR e.1) (GPRVal.denote ctx.gpr e.2 (StateVar.denote ctx.state prev_state))
+    (Expr.denote_writes ctx us prev_state) := by
+  simp only [Expr.denote_writes]
+
+theorem denote_statevar_eq_denote_writes_eq
+  (h : StateVar.denote ctx.state v1 = StateVar.denote ctx.state v2) :
+  Expr.denote_writes ctx writes v1 = Expr.denote_writes ctx writes v2 := by
+  induction writes
+  case nil => simpa [Expr.denote_writes]
+  case cons =>
+    rename_i head tail h_ind
+    simp [Expr.denote_writes]
+    simp_all only
+  done
+
+-- TODO: Generalize and move to Arm/State.
+theorem w_of_w_gpr_commute (i j : BitVec 5)
+  (h : i ≠ j) :
+  w (StateField.GPR i) v1 (w (StateField.GPR j) v2 s) =
+  w (StateField.GPR j) v2 (w (StateField.GPR i) v1 s) := by
+  simp_all [w, write_base_gpr, Update.regIndexLe]
+  unfold write_store
+  ext i
+  (repeat (split <;> simp_all!))
+  done
+
+private theorem denote_writes_sorted_helper
+  (h : ∀ (b : Update), b ∈ l1 → (!head.regIndexLe b) = true) :
+  Expr.denote_writes ctx (l1 ++ head :: l2) s =
+  Expr.denote_writes ctx (head :: l1 ++ l2) s := by
+  induction l1
+  case nil => simp_all only [List.not_mem_nil,
+                             Bool.not_eq_eq_eq_not,
+                             Bool.not_true, false_implies,
+                             implies_true, List.nil_append,
+                             denote_writes_cons,
+                             List.singleton_append]
+  case cons =>
+    rename_i head' tail' ih
+    simp [denote_writes_cons]
+    rw [ih]
+    simp only [List.cons_append, denote_writes_cons]
+    · rw [w_of_w_gpr_commute]
+      simp_all [Update.regIndexLe]
+      apply BitVec.ne_of_lt
+      simp_all
+    · simp_all only [List.mem_cons,
+                     or_true, implies_true,
+                     List.cons_append, denote_writes_cons,
+                     true_implies, Bool.not_eq_eq_eq_not,
+                     Bool.not_true, forall_eq_or_imp, Bool.not_false]
+
+/--
+Sorting `Updates xs` using `Update.regIndexLe` is immaterial to their denotation
+over `StateVar s`.
+
+-/
+@[local simp]
+theorem denote_writes_sorted :
+  Expr.denote_writes ctx (List.mergeSort xs Update.regIndexLe) s =
+  Expr.denote_writes ctx xs s := by
+  induction xs
+  case nil => simp only [List.mergeSort_nil, denote_writes_empty]
+  case cons =>
+    rename_i head tail ih
+    simp only [denote_writes_cons]
+    have ⟨l1, l2, h1, h2, h3⟩ :=
+      @List.mergeSort_cons Update Update.regIndexLe
+        (by apply Update.regIndexLe_trans)
+        (by apply Update.regIndexLe_total)
+        head tail
+    rw [h1]
+    simp_all only [Bool.not_eq_eq_eq_not,
+                   Bool.not_true,
+                   denote_writes_sorted_helper h3,
+                   List.cons_append, denote_writes_cons]
+    done
+
 
 /--
 Denote an `Expr e` to a `Prop` corresponding to `curr_state = writes[prev_state]`.
 -/
 def Expr.denote (ctx : Context) (e : Expr) : Prop :=
   StateVar.denote ctx.state e.curr_state =
-  Expr.writes.denote ctx e.writes e.prev_state
+  Expr.denote_writes ctx e.writes e.prev_state
 
 /--
 Return a `Prop` corresponding to `e1 = e2`.
@@ -162,17 +259,23 @@ def Exprs.denote (ctx : Context) (es : Exprs) : Prop :=
 def Expr.default : Expr :=
   { prev_state := 0, curr_state := 0, writes := [] }
 
+/--
+Insert `u`, which comes after `es`, at an appropriate safe point in `es`.
+
+Note that `u` only changes `es` only if it shadows some update in it.
+Independent updates are unaffected.
+-/
 def Update.insertSorted (es : Updates) (u : Update) : Updates :=
   match es with
   | [] => [u]
   | e :: rest =>
-    if u.regIndexLt e then
-      -- `u` does not appear in `es` (given that `es` is sorted), so we retain
-      -- this update.
-      u :: es
-    else if u.regEq e then
-      -- We overwrite `e` with `x`.
+    if u.regEq e then
+      -- We overwrite `e` with `u`.
       u :: rest
+    else if u.regIndexLe e then
+      -- `u` does not appear in `es` (given that `es` is
+      -- sorted). We order `u` before `e` to retain this update.
+      u :: es
     else
       e :: (insertSorted rest u)
 
@@ -192,6 +295,25 @@ def Update.resolveRead (es : Updates) (u : Update) : Update :=
     | (.w_gpr i v) :: rest =>
       if i == gpr_idx then v else go gpr_idx rest
 
+@[local simp]
+theorem Update.resolveRead_w_gpr :
+  Update.resolveRead es (.w_gpr i (.var v)) = (.w_gpr i (.var v)) := by
+  simp [Update.resolveRead]
+  done
+
+@[local simp]
+theorem Update.resolveRead_empty_1 :
+  Update.resolveRead [] u = u := by
+  simp [Update.resolveRead]
+  split <;> rfl
+
+@[local simp]
+theorem Update.resolveRead_index_unchanged (w : Updates) :
+  (Update.resolveRead w u).1 = u.1 := by
+  simp [Update.resolveRead]
+  split <;> simp only
+  done
+
 /--
 Resolve any reads in each of `us` by looking them up in `es`, which is expected
 to be sorted.
@@ -199,12 +321,55 @@ to be sorted.
 def Update.resolveReads (es us : Updates) : Updates :=
   us.map (Update.resolveRead es)
 
+@[local simp]
+theorem Update.resolveReads_cons_w_gpr :
+  Update.resolveReads es (Update.w_gpr i (GPRVal.var idx) :: tail) =
+  Update.w_gpr i (GPRVal.var idx) :: (Update.resolveReads es tail) := by
+  simp [Update.resolveReads, Update.resolveRead]
+
+@[local simp]
+theorem Update.resolveReads_empty_1 :
+  Update.resolveReads [] us = us := by
+  simp [Update.resolveReads]
+  apply List.map_id''; intro i
+  apply Update.resolveRead_empty_1
+  done
+
+@[local simp]
+theorem Update.resolvedReads_empty_2 :
+  Update.resolveReads es [] = [] := by
+  simp only [resolveReads, List.map_nil]
+
+@[local simp]
+theorem Update.resolveRead_empty_1_fn_is_id :
+  (Update.resolveRead []) = id := by
+  ext
+  simp [resolveRead]
+  split <;> simp_all [resolveRead.go]
+  done
+
+@[local simp]
+theorem map_resolveRead_empty_1 :
+  (List.map (Update.resolveRead []) us) = us := by
+  simp [Update.resolveRead_empty_1_fn_is_id]
+  done
+
+-- If a write shadows another, then `List.mergeSort` with `Update.regIndexLe`
+-- will preserve the order of the writes.
+open Expr Update in
+/--
+info: [ArmConstr.Update.w_gpr 0x01#5 (ArmConstr.GPRVal.var 1),
+ArmConstr.Update.w_gpr 0x01#5 (ArmConstr.GPRVal.var 2)]
+-/
+#guard_msgs in
+#eval List.mergeSort [.w_gpr 1#5 (.var 1), .w_gpr 1#5 (.var 2)] Update.regIndexLe
+
 /--
 Aggregate `e` and `u`, assuming `u` follows `e`.
 -/
 def Expr.aggregate1 (e u : Expr) : Expr :=
   if e.curr_state == u.prev_state then
-    let e_sorted_writes := List.mergeSort e.writes Update.regIndexLt
+    let e_sorted_writes := List.mergeSort e.writes Update.regIndexLe
     let u_resolved_writes := Update.resolveReads e_sorted_writes u.writes
     { prev_state := e.prev_state,
       curr_state := u.curr_state,
@@ -219,7 +384,19 @@ def Expr.aggregate1 (e u : Expr) : Expr :=
   | [], us => us
   | es, [] => es
   | es, u :: rest_us =>
-    go (Update.insertSorted es u) rest_us
+    Update.insertSorted (go es rest_us) u
+
+@[local simp]
+theorem Expr.aggregate1.go_empty_1 :
+  Expr.aggregate1.go [] us = us := by
+  simp [Expr.aggregate1.go]
+
+@[local simp]
+theorem Expr.aggregate1.go_empty_2 :
+  Expr.aggregate1.go es [] = es := by
+  unfold Expr.aggregate1.go
+  split <;> simp_all
+  done
 
 /--
 info: { curr_state := 2,
@@ -240,7 +417,7 @@ open Expr Update in
 
 /--
 Aggregate `es` onto `init`.
-Earlier updates appear first in `es`, and of course, `es` follows `init`.
+Earlier updates appear first in `es`, and `es` follow `init`.
 -/
 def Expr.aggregate (init : Expr) (es : Exprs) : Expr :=
   match es with
@@ -273,25 +450,190 @@ info: { curr_state := 2,
 def Expr.isAggregated (init : Expr) (updates : Exprs) (final : Expr) : Bool :=
   final == aggregate init updates
 
---
--- #check decidable_of_decidable_of_iff
+/--
+If `next.writes` is empty, then
+```
+next.curr_state = sorted(init.writes(init.prev_state))
+```
+-/
+theorem Expr.denote_when_next_writes_empty
+  (h_init : denote ctx init)
+  (h_next : denote ctx next)
+  (h_init_curr_next_prev : init.curr_state = next.prev_state)
+  (h_next_writes_empty : next.writes = []) :
+  denote ctx
+    { curr_state := next.curr_state, prev_state := init.prev_state,
+      writes := List.mergeSort init.writes Update.regIndexLe } := by
+  simp only [denote] at *
+  simp [h_next_writes_empty] at h_next
+  rw [h_next, ←h_init_curr_next_prev, h_init, denote_writes_sorted]
+  done
 
--- Hint: Reduction got stuck on '▸' (Eq.rec), which suggests that one of the
--- 'Decidable' instances is defined using tactics such as 'rw' or 'simp'. To
--- avoid tactics, make use of functions such as 'inferInstanceAs' or
--- 'decidable_of_decidable_of_iff' to alter a proposition.
+/--
+Using `Update.insertSorted es u` is equivalent to inserting `u` at the beginning
+of `es`, vis-a-vis denotation. This is because `Update.insertSorted` only
+modifies an `Update` in `es` if `u` shadows it.
+-/
+@[local simp]
+theorem denote_writes_insertSorted :
+  Expr.denote_writes ctx (Update.insertSorted es u) s =
+  Expr.denote_writes ctx (u :: es) s := by
+  induction es
+  case nil =>
+    simp [Update.insertSorted]
+  case cons =>
+    rename_i head tail ih
+    simp [Update.insertSorted]
+    split
+    case isTrue =>
+      rename_i h_u_head_eq
+      simp only [denote_writes_cons]
+      simp_all only [Update.regEq]
+      rw [h_u_head_eq, w_of_w_shadow]
+    case isFalse =>
+      rename_i h_u_head_neq
+      simp_all only [Update.regEq]
+      split
+      · simp only [denote_writes_cons]
+      · simp only [denote_writes_cons]
+        rw [ih]
+        simp only [denote_writes_cons]
+        rw [w_of_w_gpr_commute]
+        exact fun a => h_u_head_neq (id (Eq.symm a))
+  done
 
+/--
+Resolving `Update u` w.r.t. `writes` and then denoting it over `StateVar s0`
+is equivalent to denoting the _unresolved_ `u` w.r.t. `writes` denoted over
+`s0`.
+-/
+theorem GPRVal.denote_resolveRead (ctx : Context) :
+  GPRVal.denote ctx.gpr (Update.resolveRead writes u).2 (StateVar.denote ctx.state s0) =
+  GPRVal.denote ctx.gpr u.2 (Expr.denote_writes ctx writes s0) := by
+  induction writes generalizing u
+  case nil =>
+    simp only [denote_writes_empty, Update.resolveRead_empty_1]
+  case cons =>
+    rename_i head tail ih
+    simp only [denote_writes_cons]
+    simp [Update.resolveRead]
+    split
+    case h_1 =>
+      rename_i u' idx var
+      simp [GPRVal.denote_of_var]
+    case h_2 =>
+      rename_i u' i' gpr_idx
+      simp [Update.resolveRead.go]
+      split
+      case isTrue =>
+        rename_i h_eq
+        subst gpr_idx
+        simp [GPRVal.denote, r_of_w_same]
+      case isFalse =>
+        rename_i h_neq
+        conv => rhs; simp [GPRVal.denote]
+        rw [r_of_w_different (by simp_all; exact fun a => h_neq (id (Eq.symm a)))]
+        have ih' := @ih (.w_gpr gpr_idx (GPRVal.r_gpr gpr_idx))
+        simp [Update.resolveRead] at ih'
+        rw [ih']
+        simp [GPRVal.denote]
+  done
 
-/-- TODO: we're probably missing well-formedness hyps. about the `ctx` and/or
-  `updates` here. -/
-theorem Expr.eq_true_of_isValid (ctx : Context) (init final : Expr) (updates : Exprs) :
+/--
+`Expr.aggregate1` aggregates `first` and `second` correctly, allowing
+us to express `second.curr_state` in terms of `first.prev_state`. That is:
+```
+if first.curr_state = first.writes[first.prev_state] and
+   second.curr_state = second.writes[second.prev_state] then
+ second.curr_state = resolveReads(second.writes, first.writes)[first.prev_state]
+```
+-/
+theorem Expr.denote_aggregate1
+  (h1 : Expr.denote ctx first)
+  (h2 : Expr.denote ctx second) :
+  Expr.denote ctx (aggregate1 first second) := by
+  simp [aggregate1]
+  by_cases h₀ : first.curr_state = second.prev_state
+  case neg => -- h0 : first.curr_state ≠ second.prev_state
+    simp_all only [minimal_theory]
+  case pos => -- first.curr_state = second.prev_state
+    simp_all [denote]
+    rw [←h₀] at h1 h2 ⊢
+    generalize first.prev_state = s0 at *
+    generalize first.curr_state = s1 at *
+    generalize first.writes = writes1 at *
+    generalize second.writes = writes2 at *
+    clear h₀ h2 first second
+    induction writes2 generalizing s0 s1 writes1
+    case nil =>
+      simp_all
+      rw [Update.resolvedReads_empty_2]
+      unfold aggregate1.go
+      split
+      · have : writes1 = [] := by
+          have := @List.length_mergeSort Update Update.regIndexLe writes1
+          simp_all only [List.length_nil]
+          exact List.length_eq_zero.mp (id (Eq.symm this))
+        simp_all only [denote_writes_empty]
+      · simp [denote_writes_sorted]
+      · simp_all
+    case cons =>
+      rename_i u us ih
+      simp [denote_writes_cons]
+      simp [Update.resolveReads]
+      conv => rhs; unfold aggregate1.go
+      split
+      case h_1 =>
+        have : writes1 = [] := by
+          have := @List.length_mergeSort Update Update.regIndexLe writes1
+          simp_all only [List.length_nil]
+          exact List.length_eq_zero.mp (id (Eq.symm this))
+        simp_all [Update.resolveRead_empty_1]
+        rw [ih s0 s1 [] h1]
+        simp [Expr.aggregate1.go_empty_1, Update.resolveReads_empty_1, map_resolveRead_empty_1]
+      case h_2 => contradiction
+      case h_3 =>
+        rename_i es' us' u' rest_us' h_eq h_nonempty
+        have h_u' : u' = Update.resolveRead (List.mergeSort writes1 Update.regIndexLe) u := by
+          simp_all
+        have h_rest_us' : rest_us' = List.map (Update.resolveRead (List.mergeSort writes1 Update.regIndexLe)) us := by
+          simp_all
+        subst u' rest_us'
+        clear h_eq
+        rw [denote_writes_insertSorted]
+        simp [denote_writes_cons]
+        rw [Update.resolveRead_index_unchanged]
+        simp [Update.resolveReads] at ih
+        rw [←ih s0 s1 writes1 h1]
+        rw [GPRVal.denote_resolveRead]
+        rw [denote_writes_sorted, h1]
+  done
+
+/--
+If `Expr.isAggregated` computes that aggregating `updates` over `init` yields
+`final`, then it accurately represents `ArmState` aggregation in logic.
+-/
+theorem Expr.eq_true_of_denote (ctx : Context) (init final : Expr) (updates : Exprs) :
   (Expr.isAggregated init updates final) →
   Expr.denote ctx init ∧ Exprs.denote ctx updates → (Expr.denote ctx final) := by
-  sorry
+  induction updates generalizing init
+  case nil =>
+    simp only [isAggregated, aggregate, beq_iff_eq, Exprs.denote, and_true]
+    intro i; simp_all only [minimal_theory]
+  case cons =>
+    rename_i head tail h_ind
+    simp [isAggregated] at *
+    simp [aggregate, Exprs.denote]
+    intros h_final h_init h_head h_tail
+    have h_aggr1 := @Expr.denote_aggregate1 ctx init head h_init h_head
+    have h_ind' := h_ind (init.aggregate1 head) h_final h_aggr1 h_tail
+    exact h_ind'
+    done
 
 -------------------------------------------------------------------------------
+-------------------------------------------------------------------------------
 
--- Tests
+-- Litmus Tests
 
 open Expr Update in
 example :  Expr.isAggregated
@@ -305,7 +647,6 @@ example :  Expr.isAggregated
       with_unfolding_all decide
 
 #time
--- set_option trace.Meta.synthInstance true in
 open Expr Update in
 theorem completely_shadowed_updates
   (h_s1 : s1 = w (.GPR 0#5) x0 (w (.GPR 1#5) x1 s0))
@@ -323,7 +664,7 @@ theorem completely_shadowed_updates
     s2 = xxxx : Prop
   -/
   s2 = w (.GPR 0#5) x0 (w (.GPR 1#5) x1 s0) := by
-  have := (Expr.eq_true_of_isValid { state := [s0, s1, s2],
+  have := (Expr.eq_true_of_denote { state := [s0, s1, s2],
                                      gpr := [x0, x1] }
           -- init
           { prev_state := 0, curr_state := 0, writes := []}
@@ -336,6 +677,12 @@ theorem completely_shadowed_updates
   simp only [Exprs.denote, List.foldl, true_and, and_true, and_imp] at this
   exact this (Eq.refl s0) h_s1 h_s2
   done
+
+/--
+info: 'ArmConstr.completely_shadowed_updates' depends on axioms: [propext,
+Classical.choice, Lean.ofReduceBool, Quot.sound]
+-/
+#guard_msgs in #print axioms completely_shadowed_updates
 
 open Expr Update in
 theorem partially_shadowed_and_new_updates
@@ -356,7 +703,7 @@ theorem partially_shadowed_and_new_updates
   -- (h_s2 : s2 = w (.GPR 1#5) x1 (w (.GPR 3#5) x3 s1)) :
   (h_s2 : s2 = w (.GPR 3#5) x3 (w (.GPR 1#5) x1 s1)) :
   s2 = w (.GPR 0#5) x0 (w (.GPR 1#5) x1 (w (.GPR 3#5) x3 s0)) := by
-  have := (Expr.eq_true_of_isValid { state := [s0, s1, s2],
+  have := (Expr.eq_true_of_denote { state := [s0, s1, s2],
                                      gpr := [x0, old_x1, x1, x3] }
           -- init
           { prev_state := 0, curr_state := 0, writes := []}
@@ -390,7 +737,7 @@ theorem read_from_prev_update_test1
   (h_s1 : s1 = w (.GPR 0#5) x0 (w (.GPR 1#5) old_x1 s0))
   (h_s2 : s2 = w (.GPR 1#5) x1 (w (.GPR 3#5) (r (.GPR 1#5) s1) s1)) :
   s2 = w (.GPR 0#5) x0 (w (.GPR 1#5) x1 (w (.GPR 3#5) old_x1 s0)) := by
-  have := (Expr.eq_true_of_isValid { state := [s0, s1, s2],
+  have := (Expr.eq_true_of_denote { state := [s0, s1, s2],
                                      gpr := [x0, old_x1, x1] }
           -- init
           { prev_state := 0, curr_state := 0, writes := []}
@@ -412,7 +759,7 @@ theorem read_from_prev_update_test2 (s0 s1 s2 : ArmState)
   (h_s1 : s1 = w (.GPR 0#5) x0 (w (.GPR 1#5) old_x1 s0))
   (h_s2 : s2 = w (.GPR 1#5) x1 (w (.GPR 3#5) (r (.GPR 5#5) s1) s1)) :
   s2 = w (.GPR 0#5) x0 (w (.GPR 1#5) x1 (w (.GPR 3#5) (r (.GPR 5#5) s0) s0)) := by
-  have := (Expr.eq_true_of_isValid { state := [s0, s1, s2],
+  have := (Expr.eq_true_of_denote { state := [s0, s1, s2],
                                      gpr := [x0, old_x1, x1] }
           -- init
           { prev_state := 0, curr_state := 0, writes := []}
@@ -545,6 +892,80 @@ info: { curr_state := 30,
             [w_gpr (8#5) (GPRVal.var 87), w_gpr (9#5) (GPRVal.var 86), w_gpr (10#5) (GPRVal.var 85),
               w_gpr (11#5) (GPRVal.var 84)] }]
 
+open Expr Update in
+#eval Expr.aggregate
+      { prev_state := 0, curr_state := 0, writes := []}
+      [  { curr_state := 1, prev_state := 0, writes := [w_gpr 13#5 (.var 1), w_gpr 14#5 (.var 0), ] },
+   { curr_state := 2, prev_state := 1, writes := [w_gpr 11#5 (.var 2), ] },
+   { curr_state := 3, prev_state := 2, writes := [w_gpr 11#5 (.var 5), w_gpr 12#5 (.var 4), w_gpr 13#5 (.var 3), ] },
+   { curr_state := 4, prev_state := 3, writes := [w_gpr 10#5 (.var 10), w_gpr 11#5 (.var 9), w_gpr 12#5 (.var 8), w_gpr 13#5 (.var 7), w_gpr 14#5 (.var 6), ] },
+   { curr_state := 5, prev_state := 4, writes := [w_gpr 21#5 (.var 14), w_gpr 22#5 (.var 13), w_gpr 23#5 (.var 12), w_gpr 24#5 (.var 11), ] },
+   { curr_state := 6, prev_state := 5, writes := [w_gpr 2#5 (.var 19), w_gpr 3#5 (.var 18), w_gpr 4#5 (.var 17), w_gpr 5#5 (.var 16), w_gpr 6#5 (.var 15), ] },
+   { curr_state := 7, prev_state := 6, writes := [w_gpr 28#5 (.var 22), w_gpr 29#5 (.var 21), w_gpr 30#5 (.var 20), ] },
+   { curr_state := 8, prev_state := 7, writes := [w_gpr 21#5 (.var 27), w_gpr 22#5 (.var 26), w_gpr 23#5 (.var 25), w_gpr 24#5 (.var 24), w_gpr 25#5 (.var 23), ] },
+   { curr_state := 9, prev_state := 8, writes := [w_gpr 29#5 (.var 28), ] },
+   { curr_state := 10, prev_state := 9, writes := [w_gpr 29#5 (.var 29), ] },
+ ]
+
+#time
+open Expr Update in
+theorem test_10_steps (s0 : ArmState)
+  (h_step_1 : s1 = (w (.GPR 13#5) val1 (w (.GPR 14#5) val0 s0)))
+  (h_step_2 : s2 = (w (.GPR 11#5) val2 s1))
+  (h_step_3 : s3 = (w (.GPR 11#5) val5 (w (.GPR 12#5) val4 (w (.GPR 13#5) val3 s2))))
+  (h_step_4 : s4 = (w (.GPR 10#5) val10 (w (.GPR 11#5) val9 (w (.GPR 12#5) val8 (w (.GPR 13#5) val7 (w (.GPR 14#5) val6 s3))))))
+  (h_step_5 : s5 = (w (.GPR 21#5) val14 (w (.GPR 22#5) val13 (w (.GPR 23#5) val12 (w (.GPR 24#5) val11 s4)))))
+  (h_step_6 : s6 = (w (.GPR 2#5) val19 (w (.GPR 3#5) val18 (w (.GPR 4#5) val17 (w (.GPR 5#5) val16 (w (.GPR 6#5) val15 s5))))))
+  (h_step_7 : s7 = (w (.GPR 28#5) val22 (w (.GPR 29#5) val21 (w (.GPR 30#5) val20 s6))))
+  (h_step_8 : s8 = (w (.GPR 21#5) val27 (w (.GPR 22#5) val26 (w (.GPR 23#5) val25 (w (.GPR 24#5) val24 (w (.GPR 25#5) val23 s7))))))
+  (h_step_9 : s9 = (w (.GPR 29#5) val28 s8))
+  (h_step_10 : s10 = (w (.GPR 29#5) val29 s9))
+  :
+  s10 = (w (.GPR  0x02#5) val19 (w (.GPR  0x03#5) val18 (w (.GPR  0x04#5) val17 (w (.GPR  0x05#5) val16 (w (.GPR  0x06#5) val15 (w (.GPR  0x0a#5) val10 (w (.GPR  0x0b#5) val9 (w (.GPR  0x0c#5) val8 (w (.GPR  0x0d#5) val7 (w (.GPR  0x0e#5) val6 (w (.GPR  0x15#5) val27 (w (.GPR  0x16#5) val26 (w (.GPR  0x17#5) val25 (w (.GPR  0x18#5) val24 (w (.GPR  0x19#5) val23 (w (.GPR  0x1c#5) val22 (w (.GPR  0x1d#5) val29 (w (.GPR  0x1e#5) val20 s0)))))))))))))))))) := by
+    have := (Expr.eq_true_of_denote
+            -- Context
+            { state := [s0, s1, s2, s3, s4, s5, s6, s7, s8, s9, s10],
+               gpr := [val0, val1, val2, val3, val4, val5, val6, val7, val8, val9, val10, val11, val12, val13, val14, val15, val16, val17, val18, val19, val20, val21, val22, val23, val24, val25, val26, val27, val28, val29] }
+            -- init
+            { curr_state := 0, prev_state := 0, writes := [] }
+            -- final
+            { curr_state := 10,
+              prev_state := 0,
+              writes := [ArmConstr.Update.w_gpr 0x02#5 (ArmConstr.GPRVal.var 19),
+                         ArmConstr.Update.w_gpr 0x03#5 (ArmConstr.GPRVal.var 18),
+                         ArmConstr.Update.w_gpr 0x04#5 (ArmConstr.GPRVal.var 17),
+                         ArmConstr.Update.w_gpr 0x05#5 (ArmConstr.GPRVal.var 16),
+                         ArmConstr.Update.w_gpr 0x06#5 (ArmConstr.GPRVal.var 15),
+                         ArmConstr.Update.w_gpr 0x0a#5 (ArmConstr.GPRVal.var 10),
+                         ArmConstr.Update.w_gpr 0x0b#5 (ArmConstr.GPRVal.var 9),
+                         ArmConstr.Update.w_gpr 0x0c#5 (ArmConstr.GPRVal.var 8),
+                         ArmConstr.Update.w_gpr 0x0d#5 (ArmConstr.GPRVal.var 7),
+                         ArmConstr.Update.w_gpr 0x0e#5 (ArmConstr.GPRVal.var 6),
+                         ArmConstr.Update.w_gpr 0x15#5 (ArmConstr.GPRVal.var 27),
+                         ArmConstr.Update.w_gpr 0x16#5 (ArmConstr.GPRVal.var 26),
+                         ArmConstr.Update.w_gpr 0x17#5 (ArmConstr.GPRVal.var 25),
+                         ArmConstr.Update.w_gpr 0x18#5 (ArmConstr.GPRVal.var 24),
+                         ArmConstr.Update.w_gpr 0x19#5 (ArmConstr.GPRVal.var 23),
+                         ArmConstr.Update.w_gpr 0x1c#5 (ArmConstr.GPRVal.var 22),
+                         ArmConstr.Update.w_gpr 0x1d#5 (ArmConstr.GPRVal.var 29),
+                         ArmConstr.Update.w_gpr 0x1e#5 (ArmConstr.GPRVal.var 20)] }
+            -- updates
+            [  { curr_state := 1, prev_state := 0, writes := [w_gpr 13#5 (.var 1), w_gpr 14#5 (.var 0), ] },
+               { curr_state := 2, prev_state := 1, writes := [w_gpr 11#5 (.var 2), ] },
+               { curr_state := 3, prev_state := 2, writes := [w_gpr 11#5 (.var 5), w_gpr 12#5 (.var 4), w_gpr 13#5 (.var 3), ] },
+               { curr_state := 4, prev_state := 3, writes := [w_gpr 10#5 (.var 10), w_gpr 11#5 (.var 9), w_gpr 12#5 (.var 8), w_gpr 13#5 (.var 7), w_gpr 14#5 (.var 6), ] },
+               { curr_state := 5, prev_state := 4, writes := [w_gpr 21#5 (.var 14), w_gpr 22#5 (.var 13), w_gpr 23#5 (.var 12), w_gpr 24#5 (.var 11), ] },
+               { curr_state := 6, prev_state := 5, writes := [w_gpr 2#5 (.var 19), w_gpr 3#5 (.var 18), w_gpr 4#5 (.var 17), w_gpr 5#5 (.var 16), w_gpr 6#5 (.var 15), ] },
+               { curr_state := 7, prev_state := 6, writes := [w_gpr 28#5 (.var 22), w_gpr 29#5 (.var 21), w_gpr 30#5 (.var 20), ] },
+               { curr_state := 8, prev_state := 7, writes := [w_gpr 21#5 (.var 27), w_gpr 22#5 (.var 26), w_gpr 23#5 (.var 25), w_gpr 24#5 (.var 24), w_gpr 25#5 (.var 23), ] },
+               { curr_state := 9, prev_state := 8, writes := [w_gpr 29#5 (.var 28), ] },
+               { curr_state := 10, prev_state := 9, writes := [w_gpr 29#5 (.var 29), ] },
+             ]
+            (by native_decide))
+    simp only [Exprs.denote, and_true, and_imp] at this
+    exact this (Eq.refl s0) h_step_1 h_step_2 h_step_3 h_step_4 h_step_5 h_step_6 h_step_7 h_step_8 h_step_9 h_step_10
+    done
+
 #time
 open Expr Update in
 theorem test_30_steps (s0 : ArmState)
@@ -581,7 +1002,7 @@ theorem test_30_steps (s0 : ArmState)
   s30 = (w (.GPR 0x01#5) val52 (w (.GPR 0x02#5) val51 (w (.GPR 0x03#5) val53 (w (.GPR 0x04#5) val76 (w (.GPR 0x05#5) val81 (w (.GPR 0x06#5) val74 (w (.GPR 0x07#5) val73 (w (.GPR 0x08#5) val87 (w (.GPR 0x09#5) val86 (w (.GPR 0x0a#5) val85 (w (.GPR 0x0b#5) val84 (w (.GPR 0x0c#5) val61 (w (.GPR 0x0d#5) val83 (w (.GPR 0x0e#5) val82 (w (.GPR 0x0f#5) val19 (w (.GPR 0x10#5) val80 (w (.GPR 0x11#5) val79 (w (.GPR 0x12#5) val78 (w (.GPR 0x13#5) val77 (w (.GPR 0x14#5) val44 (w (.GPR 0x15#5) val43 (w (.GPR 0x16#5) val42 (w (.GPR 0x17#5) val41 (w (.GPR 0x18#5) val3 (w (.GPR 0x19#5) val2 (w (.GPR 0x1a#5) val1 (w (.GPR 0x1b#5) val0 (w (.GPR 0x1c#5) val60 (w (.GPR 0x1d#5) val59 (w (.GPR 0x1e#5) val58 (w (.GPR 0x1f#5) val57 s0)))))))))))))))))))))))))))))))
   := by
   have :=
-    (Expr.eq_true_of_isValid { state := [s0, s1, s2, s3, s4, s5, s6, s7, s8, s9, s10,
+    (Expr.eq_true_of_denote { state := [s0, s1, s2, s3, s4, s5, s6, s7, s8, s9, s10,
                                          s11, s12, s13, s14, s15, s16, s17, s18, s19,
                                          s20, s21, s22, s23, s24, s25, s26, s27, s28, s29, s30],
                                gpr := [val0, val1, val2, val3, val4, val5, val6, val7, val8, val9, val10,
@@ -667,79 +1088,135 @@ theorem test_30_steps (s0 : ArmState)
   exact this (Eq.refl s0) h_step_1 h_step_2 h_step_3 h_step_4 h_step_5 h_step_6 h_step_7 h_step_8 h_step_9 h_step_10 h_step_11 h_step_12 h_step_13 h_step_14 h_step_15 h_step_16 h_step_17 h_step_18 h_step_19 h_step_20 h_step_21 h_step_22 h_step_23 h_step_24 h_step_25 h_step_26 h_step_27 h_step_28 h_step_29 h_step_30
   done
 
-open Expr Update in
-#eval Expr.aggregate
-      { prev_state := 0, curr_state := 0, writes := []}
-      [  { curr_state := 1, prev_state := 0, writes := [w_gpr 13#5 (.var 1), w_gpr 14#5 (.var 0), ] },
-   { curr_state := 2, prev_state := 1, writes := [w_gpr 11#5 (.var 2), ] },
-   { curr_state := 3, prev_state := 2, writes := [w_gpr 11#5 (.var 5), w_gpr 12#5 (.var 4), w_gpr 13#5 (.var 3), ] },
-   { curr_state := 4, prev_state := 3, writes := [w_gpr 10#5 (.var 10), w_gpr 11#5 (.var 9), w_gpr 12#5 (.var 8), w_gpr 13#5 (.var 7), w_gpr 14#5 (.var 6), ] },
-   { curr_state := 5, prev_state := 4, writes := [w_gpr 21#5 (.var 14), w_gpr 22#5 (.var 13), w_gpr 23#5 (.var 12), w_gpr 24#5 (.var 11), ] },
-   { curr_state := 6, prev_state := 5, writes := [w_gpr 2#5 (.var 19), w_gpr 3#5 (.var 18), w_gpr 4#5 (.var 17), w_gpr 5#5 (.var 16), w_gpr 6#5 (.var 15), ] },
-   { curr_state := 7, prev_state := 6, writes := [w_gpr 28#5 (.var 22), w_gpr 29#5 (.var 21), w_gpr 30#5 (.var 20), ] },
-   { curr_state := 8, prev_state := 7, writes := [w_gpr 21#5 (.var 27), w_gpr 22#5 (.var 26), w_gpr 23#5 (.var 25), w_gpr 24#5 (.var 24), w_gpr 25#5 (.var 23), ] },
-   { curr_state := 9, prev_state := 8, writes := [w_gpr 29#5 (.var 28), ] },
-   { curr_state := 10, prev_state := 9, writes := [w_gpr 29#5 (.var 29), ] },
- ]
-
 #time
 open Expr Update in
-theorem test_10_steps (s0 : ArmState)
-  (h_step_1 : s1 = (w (.GPR 13#5) val1 (w (.GPR 14#5) val0 s0)))
-  (h_step_2 : s2 = (w (.GPR 11#5) val2 s1))
-  (h_step_3 : s3 = (w (.GPR 11#5) val5 (w (.GPR 12#5) val4 (w (.GPR 13#5) val3 s2))))
-  (h_step_4 : s4 = (w (.GPR 10#5) val10 (w (.GPR 11#5) val9 (w (.GPR 12#5) val8 (w (.GPR 13#5) val7 (w (.GPR 14#5) val6 s3))))))
-  (h_step_5 : s5 = (w (.GPR 21#5) val14 (w (.GPR 22#5) val13 (w (.GPR 23#5) val12 (w (.GPR 24#5) val11 s4)))))
-  (h_step_6 : s6 = (w (.GPR 2#5) val19 (w (.GPR 3#5) val18 (w (.GPR 4#5) val17 (w (.GPR 5#5) val16 (w (.GPR 6#5) val15 s5))))))
-  (h_step_7 : s7 = (w (.GPR 28#5) val22 (w (.GPR 29#5) val21 (w (.GPR 30#5) val20 s6))))
-  (h_step_8 : s8 = (w (.GPR 21#5) val27 (w (.GPR 22#5) val26 (w (.GPR 23#5) val25 (w (.GPR 24#5) val24 (w (.GPR 25#5) val23 s7))))))
-  (h_step_9 : s9 = (w (.GPR 29#5) val28 s8))
-  (h_step_10 : s10 = (w (.GPR 29#5) val29 s9))
+theorem test_40_steps (s0 : ArmState)
+  (h_step_1 : s1 = (w (.GPR 4#5) val3 (w (.GPR 5#5) val2 (w (.GPR 6#5) val1 (w (.GPR 7#5) val0 s0)))))
+  (h_step_2 : s2 = (w (.GPR 6#5) val7 (w (.GPR 7#5) val6 (w (.GPR 8#5) val5 (w (.GPR 9#5) val4 s1)))))
+  (h_step_3 : s3 = (w (.GPR 6#5) val8 s2))
+  (h_step_4 : s4 = (w (.GPR 23#5) val11 (w (.GPR 24#5) val10 (w (.GPR 25#5) val9 s3))))
+  (h_step_5 : s5 = (w (.GPR 2#5) val12 s4))
+  (h_step_6 : s6 = (w (.GPR 22#5) val17 (w (.GPR 23#5) val16 (w (.GPR 24#5) val15 (w (.GPR 25#5) val14 (w (.GPR 26#5) val13 s5))))))
+  (h_step_7 : s7 = (w (.GPR 5#5) val19 (w (.GPR 6#5) val18 s6)))
+  (h_step_8 : s8 = (w (.GPR 23#5) val21 (w (.GPR 24#5) val20 s7)))
+  (h_step_9 : s9 = (w (.GPR 13#5) val22 s8))
+  (h_step_10 : s10 = (w (.GPR 1#5) val25 (w (.GPR 2#5) val24 (w (.GPR 3#5) val23 s9))))
+  (h_step_11 : s11 = (w (.GPR 14#5) val26 s10))
+  (h_step_12 : s12 = (w (.GPR 28#5) val27 s11))
+  (h_step_13 : s13 = (w (.GPR 15#5) val28 s12))
+  (h_step_14 : s14 = (w (.GPR 24#5) val29 s13))
+  (h_step_15 : s15 = (w (.GPR 4#5) val34 (w (.GPR 5#5) val33 (w (.GPR 6#5) val32 (w (.GPR 7#5) val31 (w (.GPR 8#5) val30 s14))))))
+  (h_step_16 : s16 = (w (.GPR 13#5) val38 (w (.GPR 14#5) val37 (w (.GPR 15#5) val36 (w (.GPR 16#5) val35 s15)))))
+  (h_step_17 : s17 = (w (.GPR 13#5) val40 (w (.GPR 14#5) val39 s16)))
+  (h_step_18 : s18 = (w (.GPR 20#5) val45 (w (.GPR 21#5) val44 (w (.GPR 22#5) val43 (w (.GPR 23#5) val42 (w (.GPR 24#5) val41 s17))))))
+  (h_step_19 : s19 = (w (.GPR 2#5) val46 s18))
+  (h_step_20 : s20 = (w (.GPR 11#5) val51 (w (.GPR 12#5) val50 (w (.GPR 13#5) val49 (w (.GPR 14#5) val48 (w (.GPR 15#5) val47 s19))))))
+  (h_step_21 : s21 = (w (.GPR 17#5) val55 (w (.GPR 18#5) val54 (w (.GPR 19#5) val53 (w (.GPR 20#5) val52 s20)))))
+  (h_step_22 : s22 = (w (.GPR 20#5) val60 (w (.GPR 21#5) val59 (w (.GPR 22#5) val58 (w (.GPR 23#5) val57 (w (.GPR 24#5) val56 s21))))))
+  (h_step_23 : s23 = (w (.GPR 9#5) val65 (w (.GPR 10#5) val64 (w (.GPR 11#5) val63 (w (.GPR 12#5) val62 (w (.GPR 13#5) val61 s22))))))
+  (h_step_24 : s24 = (w (.GPR 27#5) val67 (w (.GPR 28#5) val66 s23)))
+  (h_step_25 : s25 = (w (.GPR 2#5) val68 s24))
+  (h_step_26 : s26 = (w (.GPR 11#5) val69 s25))
+  (h_step_27 : s27 = (w (.GPR 1#5) val73 (w (.GPR 2#5) val72 (w (.GPR 3#5) val71 (w (.GPR 4#5) val70 s26)))))
+  (h_step_28 : s28 = (w (.GPR 11#5) val76 (w (.GPR 12#5) val75 (w (.GPR 13#5) val74 s27))))
+  (h_step_29 : s29 = (w (.GPR 26#5) val80 (w (.GPR 27#5) val79 (w (.GPR 28#5) val78 (w (.GPR 29#5) val77 s28)))))
+  (h_step_30 : s30 = (w (.GPR 13#5) val81 s29))
+  (h_step_31 : s31 = (w (.GPR 25#5) val82 s30))
+  (h_step_32 : s32 = (w (.GPR 7#5) val86 (w (.GPR 8#5) val85 (w (.GPR 9#5) val84 (w (.GPR 10#5) val83 s31)))))
+  (h_step_33 : s33 = (w (.GPR 5#5) val90 (w (.GPR 6#5) val89 (w (.GPR 7#5) val88 (w (.GPR 8#5) val87 s32)))))
+  (h_step_34 : s34 = (w (.GPR 9#5) val93 (w (.GPR 10#5) val92 (w (.GPR 11#5) val91 s33))))
+  (h_step_35 : s35 = (w (.GPR 8#5) val95 (w (.GPR 9#5) val94 s34)))
+  (h_step_36 : s36 = (w (.GPR 4#5) val97 (w (.GPR 5#5) val96 s35)))
+  (h_step_37 : s37 = (w (.GPR 28#5) val101 (w (.GPR 29#5) val100 (w (.GPR 30#5) val99 (w (.GPR 31#5) val98 s36)))))
+  (h_step_38 : s38 = (w (.GPR 17#5) val104 (w (.GPR 18#5) val103 (w (.GPR 19#5) val102 s37))))
+  (h_step_39 : s39 = (w (.GPR 19#5) val109 (w (.GPR 20#5) val108 (w (.GPR 21#5) val107 (w (.GPR 22#5) val106 (w (.GPR 23#5) val105 s38))))))
+  (h_step_40 : s40 = (w (.GPR 7#5) val110 s39))
   :
-  s10 = (w (.GPR  0x02#5) val19 (w (.GPR  0x03#5) val18 (w (.GPR  0x04#5) val17 (w (.GPR  0x05#5) val16 (w (.GPR  0x06#5) val15 (w (.GPR  0x0a#5) val10 (w (.GPR  0x0b#5) val9 (w (.GPR  0x0c#5) val8 (w (.GPR  0x0d#5) val7 (w (.GPR  0x0e#5) val6 (w (.GPR  0x15#5) val27 (w (.GPR  0x16#5) val26 (w (.GPR  0x17#5) val25 (w (.GPR  0x18#5) val24 (w (.GPR  0x19#5) val23 (w (.GPR  0x1c#5) val22 (w (.GPR  0x1d#5) val29 (w (.GPR  0x1e#5) val20 s0)))))))))))))))))) := by
-    have := (Expr.eq_true_of_isValid
+  s40 = w (.GPR 1#5) (val73) (w (.GPR 2#5) (val72) (w (.GPR 3#5) (val71) (w (.GPR 4#5) (val97) (w (.GPR 5#5) (val96) (w (.GPR 6#5) (val89) (w (.GPR 7#5) (val110) (w (.GPR 8#5) (val95) (w (.GPR 9#5) (val94) (w (.GPR 10#5) (val92) (w (.GPR 11#5) (val91) (w (.GPR 12#5) (val75) (w (.GPR 13#5) (val81) (w (.GPR 14#5) (val48) (w (.GPR 15#5) (val47) (w (.GPR 16#5) (val35) (w (.GPR 17#5) (val104) (w (.GPR 18#5) (val103) (w (.GPR 19#5) (val109) (w (.GPR 20#5) (val108) (w (.GPR 21#5) (val107) (w (.GPR 22#5) (val106) (w (.GPR 23#5) (val105) (w (.GPR 24#5) (val56) (w (.GPR 25#5) (val82) (w (.GPR 26#5) (val80) (w (.GPR 27#5) (val79) (w (.GPR 28#5) (val101) (w (.GPR 29#5) (val100) (w (.GPR 30#5) (val99) (w (.GPR 31#5) (val98) s0)))))))))))))))))))))))))))))) := by
+    have := (Expr.eq_true_of_denote
             -- Context
-            { state := [s0, s1, s2, s3, s4, s5, s6, s7, s8, s9, s10],
-               gpr := [val0, val1, val2, val3, val4, val5, val6, val7, val8, val9, val10, val11, val12, val13, val14, val15, val16, val17, val18, val19, val20, val21, val22, val23, val24, val25, val26, val27, val28, val29] }
+            { state := [s0, s1, s2, s3, s4, s5, s6, s7, s8, s9, s10, s11, s12, s13, s14, s15, s16, s17, s18, s19, s20, s21, s22, s23, s24, s25, s26, s27, s28, s29, s30, s31, s32, s33, s34, s35, s36, s37, s38, s39, s40],
+               gpr := [val0, val1, val2, val3, val4, val5, val6, val7, val8, val9, val10, val11, val12, val13, val14, val15, val16, val17, val18, val19, val20, val21, val22, val23, val24, val25, val26, val27, val28, val29, val30, val31, val32, val33, val34, val35, val36, val37, val38, val39, val40, val41, val42, val43, val44, val45, val46, val47, val48, val49, val50, val51, val52, val53, val54, val55, val56, val57, val58, val59, val60, val61, val62, val63, val64, val65, val66, val67, val68, val69, val70, val71, val72, val73, val74, val75, val76, val77, val78, val79, val80, val81, val82, val83, val84, val85, val86, val87, val88, val89, val90, val91, val92, val93, val94, val95, val96, val97, val98, val99, val100, val101, val102, val103, val104, val105, val106, val107, val108, val109, val110] }
             -- init
             { curr_state := 0, prev_state := 0, writes := [] }
-            -- final
-            { curr_state := 10,
+            -- final: run `Exprs.aggregate init updates` to get the following.
+            { curr_state := 40,
               prev_state := 0,
-              writes := [ArmConstr.Update.w_gpr 0x02#5 (ArmConstr.GPRVal.var 19),
-                         ArmConstr.Update.w_gpr 0x03#5 (ArmConstr.GPRVal.var 18),
-                         ArmConstr.Update.w_gpr 0x04#5 (ArmConstr.GPRVal.var 17),
-                         ArmConstr.Update.w_gpr 0x05#5 (ArmConstr.GPRVal.var 16),
-                         ArmConstr.Update.w_gpr 0x06#5 (ArmConstr.GPRVal.var 15),
-                         ArmConstr.Update.w_gpr 0x0a#5 (ArmConstr.GPRVal.var 10),
-                         ArmConstr.Update.w_gpr 0x0b#5 (ArmConstr.GPRVal.var 9),
-                         ArmConstr.Update.w_gpr 0x0c#5 (ArmConstr.GPRVal.var 8),
-                         ArmConstr.Update.w_gpr 0x0d#5 (ArmConstr.GPRVal.var 7),
-                         ArmConstr.Update.w_gpr 0x0e#5 (ArmConstr.GPRVal.var 6),
-                         ArmConstr.Update.w_gpr 0x15#5 (ArmConstr.GPRVal.var 27),
-                         ArmConstr.Update.w_gpr 0x16#5 (ArmConstr.GPRVal.var 26),
-                         ArmConstr.Update.w_gpr 0x17#5 (ArmConstr.GPRVal.var 25),
-                         ArmConstr.Update.w_gpr 0x18#5 (ArmConstr.GPRVal.var 24),
-                         ArmConstr.Update.w_gpr 0x19#5 (ArmConstr.GPRVal.var 23),
-                         ArmConstr.Update.w_gpr 0x1c#5 (ArmConstr.GPRVal.var 22),
-                         ArmConstr.Update.w_gpr 0x1d#5 (ArmConstr.GPRVal.var 29),
-                         ArmConstr.Update.w_gpr 0x1e#5 (ArmConstr.GPRVal.var 20)] }
+              writes := [ArmConstr.Update.w_gpr 0x01#5 (ArmConstr.GPRVal.var 73),
+             ArmConstr.Update.w_gpr 0x02#5 (ArmConstr.GPRVal.var 72),
+             ArmConstr.Update.w_gpr 0x03#5 (ArmConstr.GPRVal.var 71),
+             ArmConstr.Update.w_gpr 0x04#5 (ArmConstr.GPRVal.var 97),
+             ArmConstr.Update.w_gpr 0x05#5 (ArmConstr.GPRVal.var 96),
+             ArmConstr.Update.w_gpr 0x06#5 (ArmConstr.GPRVal.var 89),
+             ArmConstr.Update.w_gpr 0x07#5 (ArmConstr.GPRVal.var 110),
+             ArmConstr.Update.w_gpr 0x08#5 (ArmConstr.GPRVal.var 95),
+             ArmConstr.Update.w_gpr 0x09#5 (ArmConstr.GPRVal.var 94),
+             ArmConstr.Update.w_gpr 0x0a#5 (ArmConstr.GPRVal.var 92),
+             ArmConstr.Update.w_gpr 0x0b#5 (ArmConstr.GPRVal.var 91),
+             ArmConstr.Update.w_gpr 0x0c#5 (ArmConstr.GPRVal.var 75),
+             ArmConstr.Update.w_gpr 0x0d#5 (ArmConstr.GPRVal.var 81),
+             ArmConstr.Update.w_gpr 0x0e#5 (ArmConstr.GPRVal.var 48),
+             ArmConstr.Update.w_gpr 0x0f#5 (ArmConstr.GPRVal.var 47),
+             ArmConstr.Update.w_gpr 0x10#5 (ArmConstr.GPRVal.var 35),
+             ArmConstr.Update.w_gpr 0x11#5 (ArmConstr.GPRVal.var 104),
+             ArmConstr.Update.w_gpr 0x12#5 (ArmConstr.GPRVal.var 103),
+             ArmConstr.Update.w_gpr 0x13#5 (ArmConstr.GPRVal.var 109),
+             ArmConstr.Update.w_gpr 0x14#5 (ArmConstr.GPRVal.var 108),
+             ArmConstr.Update.w_gpr 0x15#5 (ArmConstr.GPRVal.var 107),
+             ArmConstr.Update.w_gpr 0x16#5 (ArmConstr.GPRVal.var 106),
+             ArmConstr.Update.w_gpr 0x17#5 (ArmConstr.GPRVal.var 105),
+             ArmConstr.Update.w_gpr 0x18#5 (ArmConstr.GPRVal.var 56),
+             ArmConstr.Update.w_gpr 0x19#5 (ArmConstr.GPRVal.var 82),
+             ArmConstr.Update.w_gpr 0x1a#5 (ArmConstr.GPRVal.var 80),
+             ArmConstr.Update.w_gpr 0x1b#5 (ArmConstr.GPRVal.var 79),
+             ArmConstr.Update.w_gpr 0x1c#5 (ArmConstr.GPRVal.var 101),
+             ArmConstr.Update.w_gpr 0x1d#5 (ArmConstr.GPRVal.var 100),
+             ArmConstr.Update.w_gpr 0x1e#5 (ArmConstr.GPRVal.var 99),
+             ArmConstr.Update.w_gpr 0x1f#5 (ArmConstr.GPRVal.var 98)] }
             -- updates
-            [  { curr_state := 1, prev_state := 0, writes := [w_gpr 13#5 (.var 1), w_gpr 14#5 (.var 0), ] },
-               { curr_state := 2, prev_state := 1, writes := [w_gpr 11#5 (.var 2), ] },
-               { curr_state := 3, prev_state := 2, writes := [w_gpr 11#5 (.var 5), w_gpr 12#5 (.var 4), w_gpr 13#5 (.var 3), ] },
-               { curr_state := 4, prev_state := 3, writes := [w_gpr 10#5 (.var 10), w_gpr 11#5 (.var 9), w_gpr 12#5 (.var 8), w_gpr 13#5 (.var 7), w_gpr 14#5 (.var 6), ] },
-               { curr_state := 5, prev_state := 4, writes := [w_gpr 21#5 (.var 14), w_gpr 22#5 (.var 13), w_gpr 23#5 (.var 12), w_gpr 24#5 (.var 11), ] },
-               { curr_state := 6, prev_state := 5, writes := [w_gpr 2#5 (.var 19), w_gpr 3#5 (.var 18), w_gpr 4#5 (.var 17), w_gpr 5#5 (.var 16), w_gpr 6#5 (.var 15), ] },
-               { curr_state := 7, prev_state := 6, writes := [w_gpr 28#5 (.var 22), w_gpr 29#5 (.var 21), w_gpr 30#5 (.var 20), ] },
-               { curr_state := 8, prev_state := 7, writes := [w_gpr 21#5 (.var 27), w_gpr 22#5 (.var 26), w_gpr 23#5 (.var 25), w_gpr 24#5 (.var 24), w_gpr 25#5 (.var 23), ] },
-               { curr_state := 9, prev_state := 8, writes := [w_gpr 29#5 (.var 28), ] },
-               { curr_state := 10, prev_state := 9, writes := [w_gpr 29#5 (.var 29), ] },
-             ]
+            [  { curr_state := 1, prev_state := 0, writes := [w_gpr 4#5 (.var 3), w_gpr 5#5 (.var 2), w_gpr 6#5 (.var 1), w_gpr 7#5 (.var 0), ] },
+  { curr_state := 2, prev_state := 1, writes := [w_gpr 6#5 (.var 7), w_gpr 7#5 (.var 6), w_gpr 8#5 (.var 5), w_gpr 9#5 (.var 4), ] },
+  { curr_state := 3, prev_state := 2, writes := [w_gpr 6#5 (.var 8), ] },
+  { curr_state := 4, prev_state := 3, writes := [w_gpr 23#5 (.var 11), w_gpr 24#5 (.var 10), w_gpr 25#5 (.var 9), ] },
+  { curr_state := 5, prev_state := 4, writes := [w_gpr 2#5 (.var 12), ] },
+  { curr_state := 6, prev_state := 5, writes := [w_gpr 22#5 (.var 17), w_gpr 23#5 (.var 16), w_gpr 24#5 (.var 15), w_gpr 25#5 (.var 14), w_gpr 26#5 (.var 13), ] },
+  { curr_state := 7, prev_state := 6, writes := [w_gpr 5#5 (.var 19), w_gpr 6#5 (.var 18), ] },
+  { curr_state := 8, prev_state := 7, writes := [w_gpr 23#5 (.var 21), w_gpr 24#5 (.var 20), ] },
+  { curr_state := 9, prev_state := 8, writes := [w_gpr 13#5 (.var 22), ] },
+  { curr_state := 10, prev_state := 9, writes := [w_gpr 1#5 (.var 25), w_gpr 2#5 (.var 24), w_gpr 3#5 (.var 23), ] },
+  { curr_state := 11, prev_state := 10, writes := [w_gpr 14#5 (.var 26), ] },
+  { curr_state := 12, prev_state := 11, writes := [w_gpr 28#5 (.var 27), ] },
+  { curr_state := 13, prev_state := 12, writes := [w_gpr 15#5 (.var 28), ] },
+  { curr_state := 14, prev_state := 13, writes := [w_gpr 24#5 (.var 29), ] },
+  { curr_state := 15, prev_state := 14, writes := [w_gpr 4#5 (.var 34), w_gpr 5#5 (.var 33), w_gpr 6#5 (.var 32), w_gpr 7#5 (.var 31), w_gpr 8#5 (.var 30), ] },
+  { curr_state := 16, prev_state := 15, writes := [w_gpr 13#5 (.var 38), w_gpr 14#5 (.var 37), w_gpr 15#5 (.var 36), w_gpr 16#5 (.var 35), ] },
+  { curr_state := 17, prev_state := 16, writes := [w_gpr 13#5 (.var 40), w_gpr 14#5 (.var 39), ] },
+  { curr_state := 18, prev_state := 17, writes := [w_gpr 20#5 (.var 45), w_gpr 21#5 (.var 44), w_gpr 22#5 (.var 43), w_gpr 23#5 (.var 42), w_gpr 24#5 (.var 41), ] },
+  { curr_state := 19, prev_state := 18, writes := [w_gpr 2#5 (.var 46), ] },
+  { curr_state := 20, prev_state := 19, writes := [w_gpr 11#5 (.var 51), w_gpr 12#5 (.var 50), w_gpr 13#5 (.var 49), w_gpr 14#5 (.var 48), w_gpr 15#5 (.var 47), ] },
+  { curr_state := 21, prev_state := 20, writes := [w_gpr 17#5 (.var 55), w_gpr 18#5 (.var 54), w_gpr 19#5 (.var 53), w_gpr 20#5 (.var 52), ] },
+  { curr_state := 22, prev_state := 21, writes := [w_gpr 20#5 (.var 60), w_gpr 21#5 (.var 59), w_gpr 22#5 (.var 58), w_gpr 23#5 (.var 57), w_gpr 24#5 (.var 56), ] },
+  { curr_state := 23, prev_state := 22, writes := [w_gpr 9#5 (.var 65), w_gpr 10#5 (.var 64), w_gpr 11#5 (.var 63), w_gpr 12#5 (.var 62), w_gpr 13#5 (.var 61), ] },
+  { curr_state := 24, prev_state := 23, writes := [w_gpr 27#5 (.var 67), w_gpr 28#5 (.var 66), ] },
+  { curr_state := 25, prev_state := 24, writes := [w_gpr 2#5 (.var 68), ] },
+  { curr_state := 26, prev_state := 25, writes := [w_gpr 11#5 (.var 69), ] },
+  { curr_state := 27, prev_state := 26, writes := [w_gpr 1#5 (.var 73), w_gpr 2#5 (.var 72), w_gpr 3#5 (.var 71), w_gpr 4#5 (.var 70), ] },
+  { curr_state := 28, prev_state := 27, writes := [w_gpr 11#5 (.var 76), w_gpr 12#5 (.var 75), w_gpr 13#5 (.var 74), ] },
+  { curr_state := 29, prev_state := 28, writes := [w_gpr 26#5 (.var 80), w_gpr 27#5 (.var 79), w_gpr 28#5 (.var 78), w_gpr 29#5 (.var 77), ] },
+  { curr_state := 30, prev_state := 29, writes := [w_gpr 13#5 (.var 81), ] },
+  { curr_state := 31, prev_state := 30, writes := [w_gpr 25#5 (.var 82), ] },
+  { curr_state := 32, prev_state := 31, writes := [w_gpr 7#5 (.var 86), w_gpr 8#5 (.var 85), w_gpr 9#5 (.var 84), w_gpr 10#5 (.var 83), ] },
+  { curr_state := 33, prev_state := 32, writes := [w_gpr 5#5 (.var 90), w_gpr 6#5 (.var 89), w_gpr 7#5 (.var 88), w_gpr 8#5 (.var 87), ] },
+  { curr_state := 34, prev_state := 33, writes := [w_gpr 9#5 (.var 93), w_gpr 10#5 (.var 92), w_gpr 11#5 (.var 91), ] },
+  { curr_state := 35, prev_state := 34, writes := [w_gpr 8#5 (.var 95), w_gpr 9#5 (.var 94), ] },
+  { curr_state := 36, prev_state := 35, writes := [w_gpr 4#5 (.var 97), w_gpr 5#5 (.var 96), ] },
+  { curr_state := 37, prev_state := 36, writes := [w_gpr 28#5 (.var 101), w_gpr 29#5 (.var 100), w_gpr 30#5 (.var 99), w_gpr 31#5 (.var 98), ] },
+  { curr_state := 38, prev_state := 37, writes := [w_gpr 17#5 (.var 104), w_gpr 18#5 (.var 103), w_gpr 19#5 (.var 102), ] },
+  { curr_state := 39, prev_state := 38, writes := [w_gpr 19#5 (.var 109), w_gpr 20#5 (.var 108), w_gpr 21#5 (.var 107), w_gpr 22#5 (.var 106), w_gpr 23#5 (.var 105), ] },
+  { curr_state := 40, prev_state := 39, writes := [w_gpr 7#5 (.var 110), ] }]
             (by native_decide))
     simp only [Exprs.denote, and_true, and_imp] at this
-    exact this (Eq.refl s0) h_step_1 h_step_2 h_step_3 h_step_4 h_step_5 h_step_6 h_step_7 h_step_8 h_step_9 h_step_10
+    exact this (Eq.refl s0) h_step_1 h_step_2 h_step_3 h_step_4 h_step_5 h_step_6 h_step_7 h_step_8 h_step_9 h_step_10 h_step_11 h_step_12 h_step_13 h_step_14 h_step_15 h_step_16 h_step_17 h_step_18 h_step_19 h_step_20 h_step_21 h_step_22 h_step_23 h_step_24 h_step_25 h_step_26 h_step_27 h_step_28 h_step_29 h_step_30 h_step_31 h_step_32 h_step_33 h_step_34 h_step_35 h_step_36 h_step_37 h_step_38 h_step_39 h_step_40
     done
-
 
 end ArmConstr
